Isabelle_Set/Cardinals.thy
@@ -1,0 +1,18 @@
+\<^marker>\<open>creator "Alexander Krauss"\<close>
+\<^marker>\<open>creator "Josh Chen"\<close>
+\<^marker>\<open>creator "Kevin Kappelmann"\<close>
+section\<open>Cardinals\<close>
+theory Cardinals
+  imports 
+    TFunctions
+    Ordinals
+begin
+
+term bijection_on
+
+definition "card (X :: set) \<equiv> (LEAST i. i : Ord \<and> (\<exists>(f :: set \<Rightarrow> set)(g :: set \<Rightarrow> set). 
+  bijection_on X i f g))"
+
+
+
+end
